Binary search using seq.fsi: probably faster, but Z3 needs hints anyway (it is a matter of instantiating quantifiers)

examples/algorithms/binary_search.fst
@@ -17,19 +17,7 @@
 
 module BinarySearch
 
-
-(**********************************************************************)
-(* Representation of unmutable arrays in such a way that we can       *)
-(* prove totality: a total function and the length                    *)
-(**********************************************************************)
-
-type array 'a = (int -> Tot 'a) * nat
-
-val arr : array 'a -> int -> Tot 'a
-let arr t = let (t,_) = t in t
-
-val length : array 'a -> Tot nat
-let length t = let (_,l) = t in l
+open Seq
 
 
 (* (\**********************************************************************\) *)
@@ -47,14 +35,15 @@ let length t = let (_,l) = t in l
 (* The binary search algorithm                                        *)
 (**********************************************************************)
 
-val bsearch_rec : t:(int -> Tot int) -> a:int -> i:nat -> j:int{-1 <= j}
-                  -> Tot (option int)   (decreases %[(j+1)-i])
+val bsearch_rec : t:(seq int) -> a:int
+                  -> i:nat{i <= length t} -> j:int{-1 <= j /\ j < length t}
+                  -> Tot (option (r:nat{r < length t}))   (decreases %[(j+1)-i])
 let rec bsearch_rec t a i j =
   if i > j then
     None
   else
     let mid = (i + j)/2 in
-    let b = t mid in
+    let b = index t mid in
     if b = a then               (* a = b *)
       Some mid
     else if b < a then          (* b < a *)
@@ -63,118 +52,114 @@ let rec bsearch_rec t a i j =
       bsearch_rec t a i (mid-1)
 
 
-val bsearch : t:(array int) -> int -> Tot (option int)
-let bsearch t a = bsearch_rec (arr t) a 0 ((length t)-1)
+val bsearch : t:(seq int) -> int -> Tot (option (r:nat{r < length t}))
+let bsearch t a = bsearch_rec t a 0 ((length t)-1)
 
 
 (**********************************************************************)
 (* Correctness                                                        *)
 (**********************************************************************)
 
-(* val bsearch_rec_correct : t:(int -> Tot int) *)
-(*                           -> a:int -> i:nat -> j:int{-1 <= j} *)
-(*                           -> Lemma *)
-(*                                (requires True) *)
-(*                                (ensures (is_Some (bsearch_rec t a i j) ==> *)
-(*                                            (Some.v (bsearch_rec t a i j) >= i) /\ *)
-(*                                            (Some.v (bsearch_rec t a i j) <= j) /\ *)
-(*                                            (t (Some.v (bsearch_rec t a i j)) = a))) *)
-(*                                (decreases %[(j+1)-i]) *)
-(* let rec bsearch_rec_correct t a i j = *)
-(*   if i > j then *)
-(*     () *)
-(*   else *)
-(*     let mid = (i + j)/2 in *)
-(*     let b = t mid in *)
-(*     if b = a then               (\* a = b *\) *)
-(*       () *)
-(*     else if b < a then          (\* b < a *\) *)
-(*       bsearch_rec_correct t a (mid+1) j *)
-(*     else                        (\* a < b *\) *)
-(*       bsearch_rec_correct t a i (mid-1) *)
+val bsearch_rec_correct : t:(seq int)
+                          -> a:int -> i:nat{i <= length t} -> j:int{-1 <= j /\ j < length t}
+                          -> Lemma
+                               (requires True)
+                               (ensures (is_Some (bsearch_rec t a i j) ==>
+                                           (Some.v (bsearch_rec t a i j) >= i) /\
+                                           (Some.v (bsearch_rec t a i j) <= j) /\
+                                           (index t (Some.v (bsearch_rec t a i j)) = a)))
+                               (decreases %[(j+1)-i])
+let rec bsearch_rec_correct t a i j =
+  if i > j then
+    ()
+  else
+    let mid = (i + j)/2 in
+    let b = index t mid in
+    if b = a then               (* a = b *)
+      ()
+    else if b < a then          (* b < a *)
+      bsearch_rec_correct t a (mid+1) j
+    else                        (* a < b *)
+      bsearch_rec_correct t a i (mid-1)
 
 
-(* val bsearch_correct : t:(array int) -> a:int *)
-(*                       -> Lemma *)
-(*                            (requires True) *)
-(*                            (ensures (is_Some (bsearch t a) ==> *)
-(*                                        (Some.v (bsearch t a) >= 0) /\ *)
-(*                                        (Some.v (bsearch t a) < (length t)) /\ *)
-(*                                        (arr t (Some.v (bsearch t a)) = a))) *)
-(* let bsearch_correct t a = *)
-(*   bsearch_rec_correct (arr t) a 0 ((length t)-1) *)
+val bsearch_correct : t:(seq int) -> a:int
+                      -> Lemma
+                           (requires True)
+                           (ensures (is_Some (bsearch t a) ==>
+                                       (Some.v (bsearch t a) >= 0) /\
+                                       (Some.v (bsearch t a) < (length t)) /\
+                                       (index t (Some.v (bsearch t a)) = a)))
+let bsearch_correct t a =
+  bsearch_rec_correct t a 0 ((length t)-1)
 
 
-(**********************************************************************)
-(* Completeness                                                       *)
-(**********************************************************************)
+(* (\**********************************************************************\) *)
+(* (\* Completeness                                                       *\) *)
+(* (\**********************************************************************\) *)
 
 val hint1 : y:int -> a:int -> Lemma
   (requires True)
     (ensures (forall x. (((x <= y) /\ (y < a) /\ (x = a)) ==> False)))
 let hint1 y a = ()
 
-val hint2 : t:(int -> Tot int)
-                  -> l:nat
-                  -> a:int -> mid:int
+val hint2 : t:(seq int) -> a:int -> mid:int
   -> Lemma
        (requires
-          (forall i1 i2. (0 <= i1) ==> (i1 <= i2) ==> (i2 < l) ==> (t i1 <= t i2)) /\
-          (mid < l) /\
-          (t mid < a))
+          (forall i1 i2. (0 <= i1) ==> (i1 <= i2) ==> (i2 < length t) ==> (index t i1 <= index t i2)) /\
+          (0 <= mid) /\
+          (mid < length t) /\
+          (index t mid < a))
        (ensures
-          (forall p. (((0 <= p) /\ (p < l) /\ (t p = a) /\ (p <= mid)) ==> False)))
-let hint2 t l a mid = hint1 (t mid) a
+          (forall p. (((0 <= p) /\ (p < length t) /\ (index t p = a) /\ (p <= mid)) ==> False)))
+let hint2 t a mid = hint1 (index t mid) a
 
 val hint3 : y:int -> a:int -> Lemma
   (requires True)
     (ensures (forall x. (((y <= x) /\ (a < y) /\ (x = a)) ==> False)))
 let hint3 y a = ()
 
-val hint4 : t:(int -> Tot int)
-                  -> l:nat
-                  -> a:int -> mid:int
+val hint4 : t:(seq int) -> a:int -> mid:int
   -> Lemma
        (requires
-          (forall i1 i2. (0 <= i1) ==> (i1 <= i2) ==> (i2 < l) ==> (t i1 <= t i2)) /\
+          (forall i1 i2. (0 <= i1) ==> (i1 <= i2) ==> (i2 < length t) ==> (index t i1 <= index t i2)) /\
           (0 <= mid) /\
-          (a < t mid))
+          (mid < length t) /\
+          (a < index t mid))
        (ensures
-          (forall p. (((0 <= p) /\ (p < l) /\ (t p = a) /\ (mid <= p)) ==> False)))
-let hint4 t l a mid = hint3 (t mid) a
+          (forall p. (((0 <= p) /\ (p < length t) /\ (index t p = a) /\ (mid <= p)) ==> False)))
+let hint4 t a mid = hint3 (index t mid) a
 
-val bsearch_rec_complete : t:(int -> Tot int)
-                  -> l:nat
-                  -> a:int -> i:nat -> j:int{-1 <= j}
+val bsearch_rec_complete : t:(seq int)
+                  -> a:int -> i:nat{i <= length t} -> j:int{-1 <= j /\ j < length t}
                   -> Lemma
-                       (requires (forall i1 i2. (0 <= i1) ==> (i1 <= i2) ==> (i2 < l) ==> (t i1 <= t i2)) /\
-                                 (j < l) /\
-                                 (forall p. 0 <= p ==> p < l ==> t p = a ==> p < i ==> False) /\
-                                 (forall p. 0 <= p ==> p < l ==> t p = a ==> j < p ==> False))
+                       (requires (forall i1 i2. (0 <= i1) ==> (i1 <= i2) ==> (i2 < length t) ==> (index t i1 <= index t i2)) /\
+                                 (forall p. 0 <= p ==> p < length t ==> index t p = a ==> p < i ==> False) /\
+                                 (forall p. 0 <= p ==> p < length t ==> index t p = a ==> j < p ==> False))
                        (ensures ((is_None (bsearch_rec t a i j)) ==>
-                                   (forall p. i <= p ==> p <= j ==> t p = a ==> False)))
+                                   (forall p. i <= p ==> p <= j ==> index t p = a ==> False)))
                        (decreases %[(j+1)-i])
-let rec bsearch_rec_complete t l a i j =
+let rec bsearch_rec_complete t a i j =
   if i > j then
     ()
   else
     let mid = (i + j)/2 in
-    let b = t mid in
+    let b = index t mid in
     if b = a then               (* a = b *)
       ()
     else if b < a then (        (* b < a *)
-      hint2 t l a mid;
-      bsearch_rec_complete t l a (mid+1) j
+      hint2 t a mid;
+      bsearch_rec_complete t a (mid+1) j
     ) else (                    (* a < b *)
-      hint4 t l a mid;
-      bsearch_rec_complete t l a i (mid-1)
+      hint4 t a mid;
+      bsearch_rec_complete t a i (mid-1)
     )
 
 val bsearch_complete :
-  t:(array int) -> a:int
+  t:(seq int) -> a:int
   -> Lemma
-       (requires (forall i1 i2. (0 <= i1) ==> (i1 <= i2) ==> (i2 < length t) ==> (arr t i1 <= arr t i2)))
+       (requires (forall i1 i2. (0 <= i1) ==> (i1 <= i2) ==> (i2 < length t) ==> (index t i1 <= index t i2)))
        (ensures ((is_None (bsearch t a)) ==>
-                 (forall p. 0 <= p ==> p < length t ==> arr t p = a ==> False)))
+                 (forall p. 0 <= p ==> p < length t ==> index t p <> a)))
 let bsearch_complete t a =
-  bsearch_rec_complete (arr t) (length t) a 0 ((length t)-1)
+  bsearch_rec_complete t a 0 ((length t)-1)
